Add semantics for prop eq (#254)
* Restore Semantics

* Add Completeness placeholders

* Add missing file

* Reflect comments

theories/Core/Semantic/Domain.v
@@ -5,12 +5,14 @@ From Mcltt.Core.Syntactic Require Export Syntax.
 Reserved Notation "'env'".
 
 Inductive domain : Set :=
-| d_nat : domain
-| d_pi : domain -> env -> exp -> domain
 | d_univ : nat -> domain
+| d_nat : domain
 | d_zero : domain
 | d_succ : domain -> domain
+| d_pi : domain -> env -> exp -> domain
 | d_fn : env -> exp -> domain
+| d_eq : domain -> domain -> domain -> domain
+| d_refl : domain -> domain
 | d_neut : domain -> domain_ne -> domain
 with domain_ne : Set :=
 (** Notice that the number x here is not a de Bruijn index but an absolute
@@ -20,6 +22,7 @@ with domain_ne : Set :=
 | d_var : forall (x : nat), domain_ne
 | d_app : domain_ne -> domain_nf -> domain_ne
 | d_natrec : env -> typ -> domain -> exp -> domain_ne -> domain_ne
+| d_eqrec : env -> domain -> typ -> exp -> domain -> domain -> domain_ne -> domain_ne
 with domain_nf : Set :=
 | d_dom : domain -> domain -> domain_nf
 where "'env'" := (nat -> domain).
@@ -52,14 +55,17 @@ Module Domain_Notations.
   Notation "( x )" := x (in custom domain at level 0, x custom domain at level 60) : mcltt_scope.
   Notation "'^' x" := x (in custom domain at level 0, x constr at level 0) : mcltt_scope.
   Notation "x" := x (in custom domain at level 0, x ident) : mcltt_scope.
-  Notation "'λ' ρ M" := (d_fn ρ M) (in custom domain at level 0, ρ custom domain at level 30, M custom exp at level 30) : mcltt_scope.
-  Notation "f x .. y" := (d_app .. (d_app f x) .. y) (in custom domain at level 40, f custom domain, x custom domain at next level, y custom domain at next level) : mcltt_scope.
-  Notation "'ℕ'" := d_nat (in custom domain) : mcltt_scope.
   Notation "'𝕌' @ n" := (d_univ n) (in custom domain at level 0, n constr at level 0) : mcltt_scope.
-  Notation "'Π' a ρ B" := (d_pi a ρ B) (in custom domain at level 0, a custom domain at level 30, ρ custom domain at level 0, B custom exp at level 30) : mcltt_scope.
+  Notation "'ℕ'" := d_nat (in custom domain) : mcltt_scope.
   Notation "'zero'" := d_zero (in custom domain at level 0) : mcltt_scope.
   Notation "'succ' m" := (d_succ m) (in custom domain at level 30, m custom domain at level 30) : mcltt_scope.
   Notation "'rec' m 'under' ρ 'return' P | 'zero' -> mz | 'succ' -> MS 'end'" := (d_natrec ρ P mz MS m) (in custom domain at level 0, P custom exp at level 60, mz custom domain at level 60, MS custom exp at level 60, ρ custom domain at level 60, m custom domain at level 60) : mcltt_scope.
+  Notation "'Π' a ρ B" := (d_pi a ρ B) (in custom domain at level 0, a custom domain at level 30, ρ custom domain at level 0, B custom exp at level 30) : mcltt_scope.
+  Notation "'λ' ρ M" := (d_fn ρ M) (in custom domain at level 0, ρ custom domain at level 30, M custom exp at level 30) : mcltt_scope.
+  Notation "f x .. y" := (d_app .. (d_app f x) .. y) (in custom domain at level 40, f custom domain, x custom domain at next level, y custom domain at next level) : mcltt_scope.
+  Notation "'Eq' a m n" := (d_eq a m n) (in custom domain at level 1, a custom domain at level 30, m custom domain at level 35, n custom domain at level 40) : mcltt_scope.
+  Notation "'refl' m" := (d_refl m) (in custom domain at level 1, m custom domain at level 40) : mcltt_scope.
+  Notation "'eqrec' n 'under' ρ 'as' 'Eq' a m1 m2 'return' B | 'refl' -> BR 'end'" := (d_eqrec ρ a B BR m1 m2 n) (in custom domain at level 0, a custom domain at level 30, B custom domain at level 60, BR custom domain at level 60, m1 custom domain at level 35, m2 custom domain at level 40, n custom domain at level 60) : mcltt_scope.
   Notation "'!' n" := (d_var n) (in custom domain at level 0, n constr at level 0) : mcltt_scope.
   Notation "'⇑' a m" := (d_neut a m) (in custom domain at level 0, a custom domain at level 30, m custom domain at level 30) : mcltt_scope.
   Notation "'⇓' a m" := (d_dom a m) (in custom domain at level 0, a custom domain at level 30, m custom domain at level 30) : mcltt_scope.
