theories/Core/Semantic/Readback/Definitions.v
@@ -30,6 +30,13 @@ Inductive read_nf : nat -> domain_nf -> nf -> Prop :=
      {{ Rnf ⇓ b m' in S s ↘ M }} ->
 
      {{ Rnf ⇓ (Π a ρ B) m in s ↘ λ A M }} )
+| read_nf_refl :
+  `( {{ Rtyp a in s ↘ A }} ->
+     {{ Rnf ⇓ a m' in s ↘ M' }} ->
+     {{ Rnf ⇓ (Eq a m1 m2) (refl m') in s ↘ refl A M' }} )
+| read_nf_eq_neut :
+  `( {{ Rne n in s ↘ N }} ->
+     {{ Rnf ⇓ (Eq a m1 m2) (⇑ b n) in s ↘ ⇑ N }} )
 | read_nf_neut :
   `( {{ Rne m in s ↘ M }} ->
      {{ Rnf ⇓ (⇑ a b) (⇑ c m) in s ↘ ⇑ M }} )
@@ -37,10 +44,6 @@ where "'Rnf' m 'in' s ↘ M" := (read_nf s m M) (in custom judg) : type_scope
 with read_ne : nat -> domain_ne -> ne -> Prop :=
 | read_ne_var :
   `( {{ Rne !x in s ↘ #(s - x - 1) }} )
-| read_ne_app :
-  `( {{ Rne m in s ↘ M }} ->
-     {{ Rnf n in s ↘ N }} ->
-     {{ Rne m n in s ↘ M N }} )
 | read_ne_natrec :
   `( (** Normal form of motive *)
      {{ ⟦ B ⟧ ρ ↦ ⇑! ℕ s ↘ b }} ->
@@ -59,6 +62,29 @@ with read_ne : nat -> domain_ne -> ne -> Prop :=
      {{ Rne m in s ↘ M }} ->
 
      {{ Rne rec m under ρ return B | zero -> mz | succ -> MS end in s ↘ rec M return B' | zero -> MZ | succ -> MS' end }} )
+| read_ne_app :
+  `( {{ Rne m in s ↘ M }} ->
+     {{ Rnf n in s ↘ N }} ->
+     {{ Rne m n in s ↘ M N }} )
+| read_ne_eqrec :
+  `( (** Normal form of type annotation *)
+     {{ Rtyp a in s ↘ A }} ->
+     {{ Rnf ⇓ a m1 in s ↘ M1 }} ->
+     {{ Rnf ⇓ a m2 in s ↘ M2 }} ->
+
+     (** Normal form of motive *)
+     {{ ⟦ B ⟧ ρ ↦ ⇑! a s ↦ ⇑! a (S s) ↦ ⇑! (Eq a (⇑! a s) (⇑! a (S s))) (S (S s)) ↘ b }} ->
+     {{ Rtyp b in S (S (S s)) ↘ B' }} ->
+
+     (** Normal form of BR *)
+     {{ ⟦ B ⟧ ρ ↦ ⇑! a s ↦ ⇑! a s ↦ refl (⇑! a s) ↘ bbr }} ->
+     {{ ⟦ BR ⟧ ρ ↦ ⇑! a s ↘ br }} ->
+     {{ Rnf ⇓ bbr br in S s ↘ BR' }} ->
+
+     (** Neutral form of m *)
+     {{ Rne n in s ↘ N }} ->
+
+     {{ Rne eqrec n under ρ as Eq a m1 m2 return B | refl -> BR end in s ↘ eqrec N as Eq A M1 M2 return B' | refl -> BR' end }} )
 where "'Rne' m 'in' s ↘ M" := (read_ne s m M) (in custom judg) : type_scope
 with read_typ : nat -> domain -> nf -> Prop :=
 | read_typ_univ :
@@ -74,6 +100,17 @@ with read_typ : nat -> domain -> nf -> Prop :=
      {{ Rtyp b in S s ↘ B' }} ->
 
      {{ Rtyp Π a ρ B in s ↘ Π A B' }})
+| read_typ_eq :
+  `( (** Normal form of equality type *)
+     {{ Rtyp a in s ↘ A }} ->
+
+     (** Normal form of LHS *)
+     {{ Rnf ⇓ a m1 in s ↘ M1 }} ->
+
+     (** Normal form of RHS *)
+     {{ Rnf ⇓ a m2 in s ↘ M2 }} ->
+
+     {{ Rtyp Eq a m1 m2 in s ↘ Eq A M1 M2 }})
 | read_typ_neut :
   `( {{ Rne b in s ↘ B }} ->
      {{ Rtyp ⇑ a b in s ↘ ⇑ B }})
